theories/sim/cmra.v
@@ -7,23 +7,27 @@ Set Default Proof Using "Type".
 Inductive tag_kind := tkUnique | tkPub.
 (* Ex() + Ag() *)
 Definition tagKindR := csumR (exclR unitC) (agreeR unitC).
+
 Definition to_tagKindR (tk: tag_kind) : tagKindR :=
   match tk with tkUnique => Cinl (Excl ()) | tkPub => Cinr (to_agree ()) end.
 
 Inductive call_state := csOwned (T: gset ptr_id) | csPub.
 (* Ex(ptr_id) + Ag() *)
 Definition callStateR := csumR (exclR (gsetC ptr_id)) (agreeR unitC).
+
 Definition to_callStateR (cs: call_state) : callStateR :=
   match cs with csOwned T => Cinl (Excl T) | csPub => Cinr (to_agree ()) end.
 
 Definition cmap := gmap call_id call_state.
 (* call_id ⇀ CallState *)
 Definition cmapUR := gmapUR call_id callStateR.
+
 Definition to_cmapUR (cm: cmap) : cmapUR := fmap to_callStateR cm.
 
 Definition ptrmap := gmap ptr_id (tag_kind * mem).
 (* ptr_id ⇀ TagKid x (loc ⇀ Ag(Scalar)) *)
 Definition ptrmapUR := gmapUR ptr_id (prodR tagKindR (gmapR loc (agreeR scalarC))).
+
 Definition to_heapUR (h: mem) : gmapR loc (agreeR scalarC) := fmap to_agree h.
 Definition to_ptrmapUR (pm: ptrmap) : ptrmapUR :=
   fmap (λ tm, (to_tagKindR tm.1, to_heapUR tm.2)) pm.
