theories/sim/invariant.v
@@ -1,0 +1,148 @@
+From stbor.lang Require Export lang.
+From stbor.sim Require Export cmra.
+
+Set Default Proof Using "Type".
+
+(** Public scalar relation *)
+(* No case for poison *)
+Definition arel (r: resUR) (s1 s2: scalar) : Prop :=
+  match s1, s2 with
+  | ScInt n1, ScInt n2 => n1 = n2
+  | ScFnPtr n1, ScFnPtr n2 => n1 = n2
+  | ScPtr l1 tg1, ScPtr l2 tg2 =>
+      l1 = l2 ∧ tg1 = tg2 ∧
+      match tg1 with
+      | Untagged => True
+      | Tagged t => ∃ h, r.1 !! t ≡ Some (to_tagKindR tkPub, h)
+      end
+  | _, _ => False
+  end.
+
+Fixpoint active_SRO (stk: stack) : gset ptr_id :=
+  match stk with
+  | [] => ∅
+  | it :: stk =>
+    match it.(perm) with
+    | SharedReadOnly => match it.(tg) with
+                        | Tagged t => {[t]} ∪ active_SRO stk
+                        | Untagged => active_SRO stk
+                        end
+    | _ => ∅
+    end
+  end.
+
+Definition ptrmap_inv (r: resUR) (σ: state) : Prop :=
+  ∀ (t: ptr_id) (k: tag_kind) h, r.1 !! t ≡ Some (to_tagKindR k, h) →
+  ∀ (l: loc) (s: scalar), h !! l ≡ Some (to_agree s) →
+  ∀ (stk: stack), σ.(sst) !! l = Some stk →
+  ∀ pm opro, mkItem pm (Tagged t) opro ∈ stk →
+  (* as long as the tag [t] is in the stack [stk],
+    then its heaplet [h] agree with the state [σ] *)
+  σ.(shp) !! l = Some s ∧
+  (* If [k] is Unique, then [t] must be Unique at the top of [stk]. Otherwise
+    if [k] is Pub, then [t] can be among the top SRO items. *)
+  match k with
+  | tkUnique => ∃ stk' opro', stk = mkItem Unique (Tagged t) opro' :: stk'
+  | tkPub => t ∈ active_SRO stk
+  end.
+
+Definition cmap_inv (r: resUR) (σ: state) : Prop :=
+  ∀ (c: call_id) (cs: callStateR), r.2 !! c ≡ Some cs →
+  match cs with
+  (* if c is a private call id *)
+  | Cinl (Excl T) =>
+      c ∈ σ.(scs) ∧
+      (* for any tag [t] owned by c *)
+      ∀ (t: ptr_id), t ∈ T →
+      (* that protects the heaplet [h] *)
+      ∀ k h, r.1 !! t ≡ Some (k, h) →
+      (* if [l] is in that heaplet [h] *)
+      ∀ (l: loc), l ∈ dom (gset loc) h →
+      (* then a c-protector must be in the stack of l *)
+      ∃ stk pm, σ.(sst) !! l = Some stk ∧ mkItem pm (Tagged t) (Some c) ∈ stk
+  (* if c is a public call id *)
+  | Cinr _ => True
+  | _ => False
+  end.
+
+(* [l] is private w.r.t to some tag [t] if [t] is uniquely owned and protected
+  by some call id [c] and [l] is in [t]'s heaplet [h]. *)
+Definition priv_loc (r: resUR) (l: loc) (t: ptr_id) :=
+  ∃ (c: call_id) (T: gset ptr_id) h,
+  r.2 !! c ≡ Some (Cinl (Excl T)) ∧ t ∈ T ∧
+  r.1 !! t ≡ Some (to_tagKindR tkUnique, h) ∧ l ∈ dom (gset loc) h.
+
+(** State relation *)
+Definition srel (r: resUR) (σs σt: state) : Prop :=
+  σs.(sst) = σt.(sst) ∧ σs.(snp) = σt.(snp) ∧
+  σs.(scs) = σt.(scs) ∧ σs.(snc) = σt.(snc) ∧
+  ∀ (l: loc) st, σt.(shp) !! l = Some st →
+  (∃ ss, σs.(shp) !! l = Some ss ∧ arel r ss st) ∨ (∃ (t: ptr_id), priv_loc r l t).
+
+Definition wsat (r: resUR) (σs σt: state) : Prop :=
+  ptrmap_inv r σt ∧ cmap_inv r σt ∧ srel r σs σt.
+
+(** Value relation for function arguments/return values *)
+(* Values passed among functions are public *)
+Definition vrel (r: resUR) (v1 v2: value) := Forall2 (arel r) v1 v2.
+Definition vrel_expr (r: resUR) (e1 e2: expr) :=
+  ∃ v1 v2, e1 = Val v1 ∧ e2 = Val v2 ∧ vrel r v1 v2.
+
+(* TODO: I hate these cmra operations *)
+Lemma ptrmap_inv_downward_mono (r1 r2 : resUR) σ (VAL: ✓ r2) :
+  r1 ≼ r2 → ptrmap_inv r2 σ → ptrmap_inv r1 σ.
+Proof.
+  move => Le PI t k h Eqh l s Eqs stk Eqst pm opro IN.
+  have HL1: Some (to_tagKindR k, h) ≼ r2.1 !! t.
+  { rewrite -Eqh. by apply lookup_included, prod_included, Le. }
+  apply option_included in HL1 as [?|[? [[k' h'] [? [Eq1 INCL]]]]]; [done|].
+  simplify_eq.
+  have VL2: ✓ (k', h').
+  { apply (lookup_valid_Some _ t (k', h') (proj1 VAL)). by rewrite Eq1. }
+  assert (r2.1 !! t ≡ Some (to_tagKindR k, h') ∧ h ≼ h') as [Eq2 LE2].
+  { rewrite Eq1. move : INCL => [[/= EQ1 EQ2]|LE].
+    - by rewrite EQ1 EQ2.
+    - apply prod_included in LE as [Eq%tag_kind_incl_eq ?]; [|apply VL2].
+      simpl in Eq. by rewrite Eq. }
+  have EQL: h' !! l ≡ Some (to_agree s).
+  { move : LE2 => /lookup_included /(_ l). rewrite Eqs.
+    move => /option_included [//|[x [s' [? [EqL EqR]]]]]. simplify_eq.
+    rewrite EqL. move : EqR => [<-//|].
+    destruct (to_agree_uninj s') as [ss Eqss].
+    - apply (lookup_valid_Some h' l). apply VL2. by rewrite EqL.
+    - by rewrite -Eqss to_agree_included => ->. }
+  specialize (PI _ _ _ Eq2 _ _ EQL _ Eqst _ _ IN). naive_solver.
+Qed.
+
+Lemma cmap_inv_downward_mono (r1 r2 : resUR) σ (VAL: ✓ r2) :
+  r1 ≼ r2 → cmap_inv r2 σ → cmap_inv r1 σ.
+Proof.
+  move => Le CI c cs Eqcs.
+  have HL1: Some cs ≼ r2.2 !! c.
+  { rewrite -Eqcs. by apply lookup_included, prod_included, Le. }
+  apply option_included in HL1 as [?|[cs1 [cs2 [? [Eq1 INCL]]]]]; [done|].
+  simplify_eq.
+  specialize (CI c cs2 (ltac: (by rewrite Eq1))).
+  have VL2: ✓ cs2.
+  { eapply (lookup_valid_Some r2.2 c). apply VAL. by rewrite Eq1. }
+  have VL1: ✓ cs1. { move : INCL => [-> //|]. by apply cmra_valid_included. }
+  destruct cs1 as [[T|]| |]; [|done..].
+  destruct INCL as [INCL|INCL]; last first.
+  { exfalso. apply (exclusive_included _ _ INCL VL2). }
+  destruct cs2 as [[T2|]| |]; [|done|by inversion INCL|done].
+  apply Cinl_inj, Excl_inj, leibniz_equiv_iff in INCL. subst T2.
+  destruct CI as [IN EQM]. split; [done|].
+  intros t INt k h Eqh l InD.
+  have HL1: Some (k, h) ≼ r2.1 !! t.
+  { rewrite -Eqh. by apply lookup_included, prod_included, Le. }
+  apply option_included in HL1 as [?|[? [[k' h'] [? [Eq2 INCL]]]]]; [done|].
+  simplify_eq.
+  have VL3: ✓ (k', h').
+  { apply (lookup_valid_Some _ t (k', h') (proj1 VAL)). by rewrite Eq2. }
+  assert (r2.1 !! t ≡ Some (k, h') ∧ h ≼ h') as [Eq3 LE2].
+  { rewrite Eq2. move : INCL => [[/= EQ1 EQ2]|LE].
+    - by rewrite EQ1 EQ2.
+    - apply prod_included in LE as [Eq%tag_kind_incl_eq ?]; [|apply VL3].
+      simpl in Eq. by rewrite Eq. }
+  apply (EQM _ INt k h' Eq3 l). eapply dom_included; eauto.
+Qed.
